@prefix rdf: <http://www.w3.org/1999/02/22-rdf-syntax-ns#> .
@prefix owl: <http://www.w3.org/2002/07/owl#> .
@prefix rdfs: <http://www.w3.org/2000/01/rdf-schema#> .
@prefix skos: <http://www.w3.org/2004/02/skos/core#> .
@prefix xsd: <http://www.w3.org/2001/XMLSchema#> .
@prefix qudt: <http://qudt.org/schema/qudt/> .
@prefix quantitykind: <https://qudt.org/2.1/vocab/quantitykind/> .
@prefix unit: <http://qudt.org/vocab/unit/> .
@prefix efkpis: <http://example.org/efkpis#> .

# Classes
efkpis:KPI rdf:type owl:Class .
efkpis:Stakeholder rdf:type owl:Class .
efkpis:DOEFlexibilityCategory rdf:type owl:Class .
efkpis:Complexity rdf:type owl:Class .
efkpis:Relevance rdf:type owl:Class .
efkpis:PerformanceAspect rdf:type owl:Class .
efkpis:SpatialResolution rdf:type owl:Class .
efkpis:TimePeriod rdf:type owl:Class ;
    rdfs:subClassOf quantitykind:Period .

efkpis:InputVariable rdf:type owl:Class .
efkpis:SingleValueInputVariable rdf:type owl:Class ;
    rdfs:subClassOf efkpis:InputVariable .
efkpis:SerialValueInputVariable rdf:type owl:Class ;
    rdfs:subClassOf efkpis:InputVariable .

# Properties
# ------------------------------------------------------------------------------
## Datatype Properties
# ------------------------------------------------------------------------------
efkpis:hasRelevance rdf:type owl:DatatypeProperty ;
    rdfs:range xsd:string .

efkpis:needsBaseline rdf:type owl:DatatypeProperty ;
    rdfs:range xsd:boolean .

efkpis:temporalResolution rdf:type owl:DatatypeProperty ;
    rdfs:range xsd:string .

efkpis:acronym rdf:type owl:DatatypeProperty ;
    rdfs:range xsd:string .

efkpis:startTime rdf:type owl:DatatypeProperty ;
    rdfs:domain efkpis:TimePeriod ;
    rdfs:range xsd:dateTime .

efkpis:endTime rdf:type owl:DatatypeProperty ;
    rdfs:domain efkpis:TimePeriod ;
    rdfs:range xsd:dateTime .

efkpis:hasValue rdf:type owl:DatatypeProperty ;
    rdfs:domain efkpis:SingleValueInputVariable ;
    rdfs:range rdfs:Literal .  # Broad range to include all literal types

efkpis:hasValues rdf:type owl:DatatypeProperty ;
    rdfs:domain efkpis:SerialValueInputVariable ;
    rdfs:range rdf:List .  # A list to represent an array of various types of data

efkpis:temporalResolutionValue rdf:type owl:DatatypeProperty ;
    rdfs:domain efkpis:InputVariable ;
    rdfs:range xsd:integer .  # Temporal resolution value as an integer

efkpis:physicalQuantity rdf:type owl:ObjectProperty ;
    rdfs:domain efkpis:InputVariable ;
    rdfs:range [ rdf:type owl:Class ;
                 owl:unionOf (qudt:QuantityKind qudt:DateTimeStringEncodingType) ] . # Linking to QUDT's class

efkpis:filePath rdf:type owl:DatatypeProperty ;
    rdfs:domain rdf:Description ;
    rdfs:range xsd:string .

efkpis:fileFormat rdf:type owl:DatatypeProperty ;
    rdfs:domain rdf:Description ;
    rdfs:range xsd:string .

efkpis:dataColumns rdf:type owl:DatatypeProperty ;
    rdfs:domain rdf:Description ;
    rdfs:range xsd:string .


# ------------------------------------------------------------------------------
## Object Properties
# ------------------------------------------------------------------------------
efkpis:hasUnit rdf:type owl:ObjectProperty ;
    rdfs:domain [ rdf:type owl:Class ;
                  owl:unionOf (efkpis:KPI efkpis:InputVariable) ] ;
    rdfs:range qudt:Unit .  # Using QUDT Unit class


efkpis:hasComplexity rdf:type owl:ObjectProperty ;
    rdfs:domain efkpis:KPI ;
    rdfs:range efkpis:Complexity .

efkpis:hasRelevance rdf:type owl:ObjectProperty ;
    rdfs:domain efkpis:KPI ;
    rdfs:range efkpis:Relevance .

efkpis:hasInterestIn rdf:type owl:ObjectProperty ;
    rdfs:domain efkpis:Stakeholder ;
    rdfs:range efkpis:KPI ;
    owl:inverseOf efkpis:hasStakeholder .

efkpis:hasStakeholder rdf:type owl:ObjectProperty ;
    rdfs:domain efkpis:KPI ;
    rdfs:range efkpis:Stakeholder ;
    owl:inverseOf efkpis:hasInterestIn .

efkpis:hasSpatialResolution rdf:type owl:ObjectProperty ;
    rdfs:domain efkpis:KPI ;
    rdfs:range efkpis:SpatialResolution .

efkpis:doeFlexibilityCategory rdf:type owl:ObjectProperty ;
    rdfs:domain efkpis:KPI ;
    rdfs:range efkpis:DOEFlexibilityCategory .

efkpis:hasPerformanceAspect rdf:type owl:ObjectProperty ;
    rdfs:domain efkpis:KPI ;
    rdfs:range efkpis:PerformanceAspect .

efkpis:hasEvaluationWindow rdf:type owl:ObjectProperty ;
    rdfs:domain efkpis:KPI ;
    rdfs:range efkpis:EvaluationWindow .

efkpis:hasInputVariable rdf:type owl:ObjectProperty ;
    rdfs:domain efkpis:KPI ;
    rdfs:range efkpis:InputVariable .

efkpis:temporalResolutionUnit rdf:type owl:ObjectProperty ;
    rdfs:domain efkpis:InputVariable ;
    rdfs:range owl:Individual .  # General range to accommodate individual OM units

efkpis:dataSource rdf:type owl:ObjectProperty ;
    rdfs:domain efkpis:SerialValueInputVariable ;
    rdfs:range rdfs:Resource .  # General range to include any type of resource

# ------------------------------------------------------------------------------
## Complexity Instances
# ------------------------------------------------------------------------------
efkpis:LowComplexity rdf:type efkpis:Complexity ;
    skos:definition "Indicates minimal data collection, processing, and calculation complexity." .

efkpis:MediumComplexity rdf:type efkpis:Complexity ;
    skos:definition "Indicates moderate data collection, processing, and calculation complexity." .

efkpis:HighComplexity rdf:type efkpis:Complexity ;
    skos:definition "Indicates significant data collection, processing, and calculation complexity, often requiring advanced computational resources or expertise." .

# ------------------------------------------------------------------------------
## Relevance Instances
# ------------------------------------------------------------------------------
efkpis:LowRelevance rdf:type efkpis:Relevance ;
    skos:definition "Indicates a lower significance or impact of the KPI in decision-making or operational contexts." .

efkpis:MediumRelevance rdf:type efkpis:Relevance ;
    skos:definition "Indicates a moderate level of significance or impact of the KPI, balancing importance with other factors in decision-making or operations." .

efkpis:HighRelevance rdf:type efkpis:Relevance ;
    skos:definition "Indicates a high significance or impact of the KPI, often critical for decision-making or operational efficiency." .


# ------------------------------------------------------------------------------
## Stakeholder Instances
# ------------------------------------------------------------------------------
## BuildingOperator
efkpis:BuildingOperator rdf:type efkpis:Stakeholder ;
    rdfs:definition "An individual or entity responsible for the operational management of a building." ;
    efkpis:hasInterestIn efkpis:FlexibilityFactor .

## Researcher
efkpis:Researcher rdf:type efkpis:Stakeholder ;
    rdfs:definition "An individual or entity conducting research in areas related to energy flexibility and building performance." ;
    efkpis:hasInterestIn efkpis:FlexibilityFactor .

## Distribution System Operator
efkpis:DistributionSystemOperator rdf:type efkpis:Stakeholder ;
    rdfs:definition "An entity responsible for operating, maintaining, and developing the distribution network of an electrical power system, ensuring safe and reliable delivery of electricity to consumers. They manage the distribution grid's infrastructure and work on integrating various energy sources and new technologies." ;
    efkpis:hasInterestIn efkpis:PeakPowerReduction .

## Transmission System Operator
efkpis:TransmissionSystemOperator rdf:type efkpis:Stakeholder ;
    rdfs:definition "An entity responsible for the high-voltage transmission of electrical power across large distances. They ensure the efficient and reliable transfer of electricity from generation facilities to distribution system operators, balancing electricity supply and demand, and maintaining grid stability." ;
    efkpis:hasInterestIn efkpis:PeakPowerReduction .


# ------------------------------------------------------------------------------
## Spatial Resolution Instances
# ------------------------------------------------------------------------------
efkpis:BuildingLevel rdf:type efkpis:SpatialResolution ;
    skos:definition "Indicates that the KPI is measured at the level of individual buildings." .

efkpis:CommunityLevel rdf:type efkpis:SpatialResolution ;
    skos:definition "Indicates that the KPI is measured at the community level, encompassing multiple buildings or infrastructure elements." .

efkpis:CityLevel rdf:type efkpis:SpatialResolution ;
    skos:definition "Indicates that the KPI is measured at the city level, reflecting urban-scale considerations." .

efkpis:NationalLevel rdf:type efkpis:SpatialResolution ;
    skos:definition "Indicates that the KPI is measured at the national level, encompassing country-wide data and implications." .

efkpis:UnspecifiedLevel rdf:type efkpis:SpatialResolution ;
    skos:definition "Indicates that the spatial scope or level of the KPI is not specifically defined or restricted. This may be used in cases where the KPI is applicable across various spatial scales or when the spatial resolution is not a determining factor in its calculation or relevance." .


# ------------------------------------------------------------------------------
## DOE Flexibility Category Instances
# ------------------------------------------------------------------------------
# DOE Flexibility Categories
efkpis:Efficiency rdf:type efkpis:DOEFlexibilityCategory ;
    skos:definition "Refers to strategies or solutions aimed at improving energy efficiency, often through optimized usage or reduced wastage." .

efkpis:Shed rdf:type efkpis:DOEFlexibilityCategory ;
    skos:definition "Involves temporarily reducing energy use in response to a demand response event or high price periods to alleviate grid stress." .

efkpis:Shift rdf:type efkpis:DOEFlexibilityCategory ;
    skos:definition "Entails shifting energy use to different times, typically from peak to off-peak periods, to balance demand and supply." .

efkpis:Modulation rdf:type efkpis:DOEFlexibilityCategory ;
    skos:definition "Refers to the ability to modulate energy usage dynamically in response to grid conditions or renewable energy availability." .

efkpis:Generation rdf:type efkpis:DOEFlexibilityCategory ;
    skos:definition "Pertains to the generation aspect of energy flexibility, focusing on adaptable and responsive energy production, often from renewable sources." .

# ------------------------------------------------------------------------------
## Performance Aspect Instances
# ------------------------------------------------------------------------------
efkpis:PowerPerformance rdf:type efkpis:PerformanceAspect ;
    skos:definition "Relates to the power-related performance of a system, focusing on aspects like peak power demand, load leveling, and power quality." .

efkpis:EnergyPerformance rdf:type efkpis:PerformanceAspect ;
    skos:definition "Concerns the energy usage efficiency and optimization, including total energy consumption and energy savings." .

efkpis:CostPerformance rdf:type efkpis:PerformanceAspect ;
    skos:definition "Focuses on the economic aspects, aiming to reduce costs associated with energy consumption and operation." .

efkpis:EmissionPerformance rdf:type efkpis:PerformanceAspect ;
    skos:definition "Targets the reduction of greenhouse gas emissions and environmental impact, aligning with sustainability goals." .

efkpis:ComfortPerformance rdf:type efkpis:PerformanceAspect ;
    skos:definition "Pertains to maintaining or enhancing occupant comfort in terms of temperature, air quality, and other environmental factors." .



# ------------------------------------------------------------------------------
## KPI Instances
# ------------------------------------------------------------------------------
## FlexibilityFactor
efkpis:FlexibilityFactor rdf:type efkpis:KPI ;
    rdfs:label "Flexibility Factor" ;
    skos:definition "Indicator of a quantity (e.g., energy, cost, emissions) during high load hours versus during low load hours, which ranges between -1 (quantity was only during high load hours) and 1 (quantity was only during low load hours)." ;
    efkpis:acronym "FF" ;
    efkpis:hasUnit unit:FRACTION;
    efkpis:hasRelevance efkpis:HighRelevance ;
    efkpis:hasComplexity efkpis:LowComplexity ;
    efkpis:needsBaseline false ;
    efkpis:hasStakeholder efkpis:BuildingOperator, efkpis:Researcher ;
    efkpis:hasEvaluationWindow efkpis:EvaluationWindow ;  # Instance of EvaluationWindow
    efkpis:hasSpatialResolution efkpis:BuildingLevel ;
    efkpis:doeFlexibilityCategory efkpis:Shift ;
    efkpis:hasPerformanceAspect efkpis:EnergyPerformance, efkpis:PowerPerformance ;
    efkpis:hasInputVariable efkpis:GenericLoadProfile, efkpis:HighLoadStartTimestamp, efkpis:HighLoadEndTimestamp .  # Example input variable instances


## PeakPowerReduction
efkpis:PeakPowerReduction rdf:type efkpis:KPI ;
    rdfs:label "Peak Power Reduction" ;
    skos:definition "Reduced power demand during peak hour due to flexible operation. The evaluation window should consider the peak hour after the flexible operation." ;
    efkpis:acronym "PPR" ;
    efkpis:hasUnit unit:KiloW ;  # Assuming use of qudt ontology for unit
    efkpis:hasRelevance efkpis:HighRelevance ;
    efkpis:hasComplexity efkpis:LowComplexity ;
    efkpis:needsBaseline true ;
    efkpis:hasStakeholder efkpis:DistributionSystemOperator, efkpis:TransmissionSystemOperator ;
    efkpis:hasEvaluationWindow efkpis:SingleEventEvaluationWindow ;  # Assuming this is an instance of efkpis:TimePeriod
    efkpis:hasSpatialResolution efkpis:UnspecifiedLevel ;
    efkpis:doeFlexibilityCategory efkpis:LoadShedding ;
    efkpis:hasPerformanceAspect efkpis:PowerPerformance ;
    # efkpis:hasInputVariable efkpis:BaselineElectricPowerProfile, efkpis:FlexibleElectricPowerProfile .
    efkpis:hasInputVariable efkpis:BaselineElectricPowerProfile, efkpis:FlexibleElectricPowerProfile, efkpis:PeakTimestamp .

    # NOTE: Question: how "smart" should we make the python function? Should it be able to detect the peak hour automatically, or manual input only?


# ------------------------------------------------------------------------------
## Time Period Instances
# ------------------------------------------------------------------------------
efkpis:EvaluationWindow rdf:type efkpis:TimePeriod ;
    efkpis:startTime "___"^^xsd:dateTime ;  # Placeholder for actual start time
    efkpis:endTime "___"^^xsd:dateTime .    # Placeholder for actual end time


# ------------------------------------------------------------------------------
## Input Variable Instances
# ------------------------------------------------------------------------------
# ~~~~~~~~~~~~ Single Value Input Variables ~~~~~~~~~~~~
## HighLoadStartTimestamp
efkpis:HighLoadStartTimestamp rdf:type efkpis:SingleValueInputVariable ;
    rdfs:label "HighLoadStartTimestamp" ;
    skos:definition "The datetime when unit price/emission are higher, or the start of the peak hours." ;
    efkpis:physicalQuantity qudt:DATETIME ;  # Using QUDT ontology for datetime encoding
    efkpis:hasValue "___"^^xsd:dateTime .  # Placeholder for actual peak datetime value

    # NOTE: we can add data source properties for input variables (e.g., Brick model, CSV file, etc.), this should be consistent with the config file.

## HighLoadEndTimestamp
efkpis:HighLoadEndTimestamp rdf:type efkpis:SingleValueInputVariable ;
    rdfs:label "HighLoadEndTimestamp" ;
    skos:definition "The datetime when unit price/emission revert to normal, or the end of the peak hours." ;
    efkpis:physicalQuantity qudt:DATETIME ;  # Representing the physical quantity as 'time'
    efkpis:hasValue "___"^^xsd:dateTime .  # Placeholder for actual datetime

## Peak Timestamp
efkpis:PeakTimestamp rdf:type efkpis:SingleValueInputVariable ;
    rdfs:label "Peak Timestamp" ;
    skos:definition "The specific datetime marking the peak of electric power demand, used to identify peak load conditions." ;
    efkpis:physicalQuantity qudt:DATETIME ;  # Representing the physical quantity as 'time'
    efkpis:hasValue "___"^^xsd:dateTime .  # Placeholder for actual peak datetime value

# ~~~~~~~~~~~~ Serial Value Input Variables ~~~~~~~~~~~~
## GenericLoadProfile
efkpis:GenericLoadProfile rdf:type efkpis:SerialValueInputVariable  ;
    rdfs:label "GenericLoadProfile" ;
    skos:definition "A generic time series of energy, cost, or GHG emissions, measured in uncontrolled (unspecified) conditions." ;
    efkpis:physicalQuantity quantitykind:Energy ;  # Representing the physical quantity (e.g., energy, cost, emissions)
    efkpis:hasUnit unit:KiloW-HR ;  # Assuming use of qudt ontology for unit
    efkpis:temporalResolutionUnit unit:SEC ;  # Referencing OM unit for second, this can be changed to other units (e.g., unit:HR, unit:DAY)
    efkpis:temporalResolutionValue "___"^^xsd:integer ;  # Placeholder for actual temporal resolution value
    efkpis:startTime "___"^^xsd:dateTime ;  # Placeholder for actual start time
    efkpis:endTime "___"^^xsd:dateTime ;    # Placeholder for actual end time
    efkpis:dataDescription _:genericLoadProfileDataSource .

## Baseline Electric Power Profile
efkpis:BaselineElectricPowerProfile rdf:type efkpis:SerialValueInputVariable  ;
    rdfs:label "Baseline Electric Power Profile" ;
    skos:definition "A time series representing the electric power profile under normal (non-flexible) operation conditions, used as a baseline for comparison." ;
    efkpis:physicalQuantity quantitykind:ElectricPower ;  # Representing the physical quantity as 'time'
    efkpis:hasUnit unit:KiloW ;  # Assuming use of qudt ontology for unit
    efkpis:temporalResolutionUnit unit:SEC ;  # Referencing OM unit for second, this can be changed to other units (e.g., unit:HR, unit:DAY)
    efkpis:temporalResolutionValue "___"^^xsd:integer ;  # Placeholder for actual temporal resolution value
    efkpis:startTime "___"^^xsd:dateTime ;  # Placeholder for actual start time
    efkpis:endTime "___"^^xsd:dateTime ;    # Placeholder for actual end time
    efkpis:dataDescription _:baselinePowerProfileDataSource .

## Flexible Electric Power Profile
efkpis:FlexibleElectricPowerProfile rdf:type efkpis:SerialValueInputVariable  ;
    rdfs:label "Flexible Electric Power Profile" ;
    skos:definition "A time series representing the electric power profile during flexible operation, reflecting changes due to demand response or other flexibility strategies." ;
    efkpis:physicalQuantity quantitykind:ElectricPower ;  # Representing the physical quantity as 'time'
    efkpis:hasUnit unit:KiloW ;  # Assuming use of qudt ontology for unit
    efkpis:temporalResolutionUnit unit:SEC ;  # Referencing OM unit for second, this can be changed to other units (e.g., unit:HR, unit:DAY)
    efkpis:temporalResolutionValue "___"^^xsd:integer ;  # Placeholder for actual temporal resolution value
    efkpis:startTime "___"^^xsd:dateTime ;  # Placeholder for actual start time
    efkpis:endTime "___"^^xsd:dateTime ;    # Placeholder for actual end time
    efkpis:dataDescription _:flexiblePowerProfileDataSource .


_:genericLoadProfileDataSource rdf:type rdf:Description ;
    efkpis:filePath "file:///path/to/generic_load_profile.csv" ;
    efkpis:fileFormat "CSV" ;
    efkpis:dataColumns "timestamp, value" .

_:baselinePowerProfileDataSource rdf:type rdf:Description ;
    efkpis:filePath "file:///path/to/dummy_power_profile.csv" ;
    efkpis:fileFormat "CSV" ;
    efkpis:dataColumns "timestamp, baselinePower (kW)" .

_:flexiblePowerProfileDataSource rdf:type rdf:Description ;
    efkpis:filePath "file:///path/to/dummy_power_profile.csv" ;
    efkpis:fileFormat "CSV" ;
    efkpis:dataColumns "timestamp, flexiblePower (kW)" .

    # NOTE: in order to map the semantic data model with the config file, we should ensure the field names are consistent in the config file.
